lib/Lib.IntTypes.Intrinsics.fsti
@@ -17,15 +17,17 @@ val add_carry_u64: cin:uint64 -> x:uint64 -> y:uint64 -> r:lbuffer uint64 (size 
       (let r = Seq.index (as_seq h1 r) 0 in 
        v r + v c * pow2 64 == v x + v y + v cin))
 
+
+(*The precondition  v x + v y + v cin <= pow2 64 - 1 comes from the fact that we except the carry value to be equal to 0 *)
 noextract
 val add_carry_u64_void: cin:uint64 -> x:uint64 -> y:uint64 -> r:lbuffer uint64 (size 1) -> 
   Stack unit 
-    (requires fun h -> live h r /\ v cin <= 1)
-    (ensures  fun h0 _ h1 -> 
-      modifies1 r h0 h1 /\ (
-      let r = Seq.index (as_seq h1 r) 0 in 
-       v r == v x + v y + v cin))
-
+  (requires fun h -> live h r /\ v cin <= 1)
+  (ensures  fun h0 _ h1 -> modifies1 r h0 h1 /\ (
+    let r = Seq.index (as_seq h1 r) 0 in 
+    v r == (v x + v y + v cin) % pow2 64
+  )
+)
 
 noextract
 val sub_borrow_u64: cin:uint64 -> x:uint64 -> y:uint64 -> r:lbuffer uint64 (size 1) -> 
@@ -36,11 +38,11 @@ val sub_borrow_u64: cin:uint64 -> x:uint64 -> y:uint64 -> r:lbuffer uint64 (size
       (let r = Seq.index (as_seq h1 r) 0 in 
        v r - v c * pow2 64 == v x - v y - v cin))
 
-
+(* The precondition v x >= v y + v cin comes from the fact that we expect the return value to be equal to 0  *)
 noextract
-val sub_borrow_u64_void: cin:uint64 -> x:uint64 -> y:uint64 -> r:lbuffer uint64 (size 1) -> 
+val sub_borrow_u64_void: cin: uint64 -> x:uint64 -> y:uint64 -> r:lbuffer uint64 (size 1) -> 
   Stack unit
-    (requires fun h -> live h r /\ v cin <= 1)
+    (requires fun h -> live h r /\ v cin <= 1 /\ v x >= v y + v cin)
     (ensures  fun h0 _ h1 -> 
       modifies1 r h0 h1 /\ 
       (let r = Seq.index (as_seq h1 r) 0 in 
